imp_system/mem/MemA.v
@@ -275,9 +275,10 @@ Section PROOF.
 
   Definition InitCond : Sk.t -> iProp :=
     fun sk => initial_mem csl sk.
-  
+
+  Variable ginv: Sk.t -> invspec.
   Variable GlobalStb: Sk.t -> gname -> option fspec.
-  Definition t : HMod.t := Seal.sealing "ccr" (SMod.to_hmod GlobalStb Mod).
+  Definition t : HMod.t := Seal.sealing "ccr" (SMod.to_hmod ginv GlobalStb Mod).
   
 End PROOF.
 End MemA.
